stuck at same

experiments/DeeperShallowEmbedding.fst
@@ -16,17 +16,22 @@ let typ1 = fun (cs:ctx) -> cs -> Type u#1
 let typ2 = fun (cs:ctx) -> cs -> Type u#2
 let typ3 = fun (cs:ctx) -> cs -> Type u#3
 
-val var : (cs : ctx)  -> typ cs -> Type u#4
-let var cs t = (c:cs) -> t c
-
 val term : (cs : ctx) -> typ cs -> Type u#4
 let term cs t = (c:cs) -> t c
 
 val empty_ctx : ctx
 let empty_ctx : ctx = raise_t empty // or true?
-
 val cons : (cs : ctx) -> typ cs -> ctx
 let cons cs t = 
-  // TODO: why is this failing?
-  either u#4 u#4 cs t
+  cs * (c:cs -> t c)
 
+val var : (cs : ctx)  -> typ cs -> Type u#4
+let var cs t = (c:cs) -> t c
+
+val weakenT : (#cs : ctx)  -> (#t : typ cs) -> typ cs -> typ (cons cs t)
+let weakenT t (c, _) = t c
+
+val same : (#cs : ctx)  -> (#t : typ cs) -> var (cons cs t) (weakenT t)
+let same = 
+  // TODO: fails here
+  fun (c, small_t) -> small_t
